frame lemma for none above w.r.t. snoc

examples/low-level/crypto/Crypto.AEAD.PRF_MAC.fst
@@ -1,11 +1,14 @@
 module Crypto.AEAD.PRF_MAC
 
+open FStar.UInt32
 open FStar.HyperStack
 open FStar.Monotonic.RRef
 
 open Crypto.Indexing
 open Flag
 open Crypto.Symmetric.PRF
+
+open Crypto.AEAD.Invariant
 
 module HS  = FStar.HyperStack
 
@@ -82,7 +85,12 @@ let prf_mac_wrapper i t k_0 x =
 (** End: prf_mac ensures prf_mac_ensures **)
 
 
-(** Start: relate prf_mac to AEAD invariant **)
+(** Start: relate prf_mac_ensures to AEAD invariant **)
+
+(*
+ * For the AEAD invariant, after prf_mac, the PRF table must contain an unused mac for the nonce,
+ * and no corresponding otp entries, further the AEAD invariant should hold
+ *)
 
 let unused_mac_exists (#i:id) (t:PRF.state i) (x:PRF.domain_mac i) (h:HS.mem) =
   safeId i ==>
@@ -91,5 +99,67 @@ let unused_mac_exists (#i:id) (t:PRF.state i) (x:PRF.domain_mac i) (h:HS.mem) =
      | None     -> False                                            //the mac entry definitely exsits in the PRF log
      | Some mac -> CMA.mac_is_unset (i, x.iv) t.mac_rgn mac h)  //it is unset
 
+private val frame_prf_find_snoc
+  (#i:id)
+  (#r:region)
+  (x:PRF.domain i)
+  (prf_table:prf_table r i)
+  (entry:entry r i)
+  (y:PRF.domain i{y `PRF.above` x}) : Lemma
+  (requires (PRF.find prf_table y == None /\ entry.x.ctr <^ x.ctr))
+  (ensures  (PRF.find (SeqProperties.snoc prf_table entry) y == None))
+let frame_prf_find_snoc #i #r x prf_table entry y = SeqProperties.find_snoc prf_table entry (is_entry_domain y)
 
+private val frame_none_above_snoc
+  (#i:id)
+  (#r:region)
+  (x:PRF.domain i)
+  (prf_table:prf_table r i)
+  (entry:entry r i) : Lemma
+  (requires (none_above x prf_table /\  
+             entry.x.ctr <^ x.ctr))
+  (ensures  (none_above x (SeqProperties.snoc prf_table entry)))
+let frame_none_above_snoc #i #r x prf_table entry =
+  let open FStar.Classical in
+  forall_intro (move_requires (frame_prf_find #i #r x prf_table entry))
 
+val inv_after_prf_mac
+  (#i:id)
+  (#rw:rw)
+  (aead_st:aead_state i rw)
+  (k_0:CMA.akey aead_st.prf.mac_rgn i)
+  (x:PRF.domain_mac i)
+  (mac:CMA.state (i,x.iv))
+  (h0 h1:mem) : Lemma
+  (requires inv aead_st h0 /\                              //invariant holds in h0
+            (safeId i ==> fresh_nonce x.iv aead_st h0) /\  //the nonce is fresh w.r.t. the AEAD table
+            prf_mac_ensures i aead_st.prf k_0 x h0 mac h1) //prf_mac_ensures holds from h0 to h1
+
+  (ensures inv aead_st h1 /\                                       //invariant holds in h1
+           (safeId i ==>  //TODO: should this be authId i??      
+             (let prf_table = HS.sel h1 (itable i aead_st.prf) in
+	      unused_mac_exists aead_st.prf x h1 /\                //unused mac exists in the prf table
+              none_above (PRF.incr i x) prf_table)))              //no otp entries exist in the prf table for this nonce
+#reset-options "--z3rlimit 100 --initial_fuel 0 --max_fuel 0 --initial_ifuel 0 --max_ifuel 0"
+let inv_after_prf_mac #i #rw aead_st k_0 x mac h0 h1 =
+  if safeId i
+  then begin
+    let aead_entries = HS.sel h0 aead_st.log in
+    let prf_table = HS.sel h0 (itable i aead_st.prf) in
+    assert (unused_aead_iv_for_prf prf_table x.iv h0);
+    assert (refines prf_table aead_entries h0);
+    frame_refines i aead_st.prf.mac_rgn prf_table aead_entries h0 h1;
+    assert (refines prf_table aead_entries h1);
+    let prf_table' = SeqProperties.snoc prf_table (PRF.Entry x mac) in
+    //TODO: we need a lemma for this assume below
+    //we need to use the pre-condition that tells us that x.iv is fresh for aead_entries
+    let b = FStar.StrongExcludedMiddle.strong_excluded_middle (h0 == h1) in
+    if b then
+      ()
+    else begin
+      assume (refines prf_table' aead_entries h1);
+      assume (unused_mac_exists aead_st.prf x h1); //from a find_snoc lemma and mac_is_unset
+      frame_none_above_snoc (PRF.incr i x) prf_table (PRF.Entry x mac);
+      //assert (none_above (PRF.incr i x) prf_table') //from initial invariant and snoc
+    end
+  end
